nit

pulse/examples/dsls/mini_steel/Pulse.Steel.Wrapper.fst
@@ -221,3 +221,7 @@ let intro_exists #a p e = fun _ -> intro_exists e p
 let while_loop inv cond body = fun _ -> while_loop inv cond body
 
 let stt_ghost_reveal a x = fun _ -> noop (); reveal x
+
+let stt_admit _ _ = admit ()
+let stt_atomic_admit _ _ = admit ()
+let stt_ghost_admit _ _ = admit ()
