pulse/examples/dsls/mini_steel/tests/Pulse.Tests.fst
@@ -173,3 +173,13 @@ let warmup (x:int) = assert (x + 1 > x)
         )
     )
 )))
+
+// %splice_t[while_test] (check ('(
+//   fun (r:ref u32) ->
+//     (expects (exists_ (fun (n:u32) -> pts_to r full_perm n)))
+//     (provides (fun _ -> pts_to r full_perm 10ul))
+//     (
+//       stt_admit (exists_ (fun (n:u32) -> pts_to r full_perm n))
+//                 fun _ -> pts_to r full_perm 10ul)
+//     )
+// )))
